pol/Polygraphs.v
@@ -17,16 +17,39 @@ Definition FreeType {F : Type} {n : nat} (X : @Augmentation F n) : Type :=
 
  *)
 
-Inductive  Aug (F : Type) (n : nat) : Type :=
-  mkAug (E : Type)  (d : E * Sphere n -> F) : Aug F n.
+Set Primitive Projections.
 
+Record Pair (A B : Type) :=
+  mkPair {
+      fst : A;
+      snd : B
+    }.
+
+Notation "x ,1" := (fst _ _ x) (at level 5).
+Notation "x ,2" := (snd _ _ x) (at level 5).
+Arguments mkPair {_ _} _ _.
+
+Notation "A × B " := (@Pair A B) (at level 20).
+
+Record Aug (F : Type) (n : nat) :=
+              mkAug {
+                  E : Type;
+                  d : E × Sphere n -> F
+                }.
+
+(* Inductive  Aug (F : Type) (n : nat) : Type := *)
+(*   mkAug (E : Type)  (d : E * Sphere n -> F) : Aug F n. *)
 
 Arguments mkAug {_ _} _ _.
+Arguments E {_ _} _.
+Arguments d {_ _} _.
+
 
 Definition FreeA {F : Type} {n : nat} (aug : Aug F n) : Type :=
-  match aug with
-  | mkAug E d =>  Pushout d (fun x  => (fst x, Faces n (snd x)) : E * Ball n)
-  end.
+  Pushout (d aug) (fun x  => mkPair (x,1) (Faces n x,2) : (E aug) × Ball n).
+  
+
+Notation "[ aug ]*" := (FreeA aug).
 
 Inductive Pol : nat -> Type :=
 |Disc : Type -> Pol 0
@@ -34,12 +57,27 @@ Inductive Pol : nat -> Type :=
 fix Free {n : nat} (P : Pol n) : Type :=
        match P with
        | Disc A => A
-       | Ext _ _ aug => FreeA aug
+       | Ext _ _ aug => [ aug ]*
        end.
 
 Opaque Free.
+Arguments Free {_} _.
 
-Notation "[ P ]*" := (Free P).
+Definition tr {n : nat} (P : Pol n) : Pol (pred n) :=
+  match P with
+  | Disc E => Disc False
+  | Ext P' aug =>  P'
+  end.
+
+
+Definition PAug {n : nat} (P : Pol n) : Aug (Free (tr P)) n :=
+  match P with
+  | Disc E => mkAug False (fun x => x,1)
+  | Ext P aug => aug
+  end.
+
+Coercion PAug : Pol >-> Aug.
+
 
 Definition case0 (P : Pol 0 -> Type) (H : forall (T : Type), P (Disc T))  (p : Pol 0) : P p := 
   match p with
@@ -47,92 +85,98 @@ Definition case0 (P : Pol 0 -> Type) (H : forall (T : Type), P (Disc T))  (p : P
   |_ => tt
   end.
 
-Definition caseS' (n : nat) (p : Pol (S n)) :
-  forall (P : Pol (S n) -> Type) (H : forall (p : Pol n) (aug : Aug [ p ]* (S n)), P (Ext p aug)), P p :=
+
+Definition caseS' {n : nat} (p : Pol (S n)) :
+  forall (P : Pol (S n) -> Type) (H : forall (p : Pol n) (aug : Aug (Free p) (S n)), P (Ext p aug)), P p :=
   match p with
   |Ext p' aug => fun P H => H p' aug
   |_ => tt
   end.
 
-(** Definition of the Morphisms of polygraphs **)
-           
-Inductive MAug {F F' : Type} {n :nat} (f : F -> F') : Aug F n -> Aug F' n -> Type :=
-  mkMAug E d E' d' (MCells: E -> E') (H : forall e x, d' (MCells e, x) = f (d (e, x))) : MAug f (mkAug E d) (mkAug E' d').
 
-Arguments mkMAug {_ _ _ _ _ _ _ _ } _ _. 
+
+
+(** Definition of the Morphisms of polygraphs **)
+
+Record MAug {F F' : Type} {n :nat} (f : F -> F') (aug : Aug F n) (aug' : Aug F' n) :=
+  mkMAug {
+      ME: E aug -> E aug';
+      Md : forall e x, d aug' (mkPair (ME e) x) = f (d aug (mkPair e x))
+    }.
+
+Arguments ME {_ _ _ _ _ aug'} _ _.
+Arguments Md {_ _ _ _ _ aug'} _ _ _.
+Arguments mkMAug {_ _ _ _ _ aug' } _ _. 
 
 Notation "aug1 - f -- aug2" := (MAug f aug1 aug2) (at level 10).  
 
 
-Definition caseMAug {F F' : Type} {n :nat} (f : F -> F') E d E' d' (Phi : (mkAug E d) - f -- (mkAug E' d')) :
-  forall (P : (mkAug E d) - f --  (mkAug E' d') -> Type)
-    (H : forall MCells HCells, P (@mkMAug F F' n f E d E' d' MCells HCells)),
-    P Phi :=
-  match Phi with
-  |mkMAug MCells HCells => (fun P H => H MCells HCells)
-  end.
+(* Definition caseMAug {F F' : Type} {n :nat} (f : F -> F') E d E' d' (Phi : (mkAug E d) - f -- (mkAug E' d')) : *)
+(*   forall (P : (mkAug E d) - f --  (mkAug E' d') -> Type) *)
+(*     (H' : forall ME HCells, P (@mkMAug F F' n f (mkAug E d) (mkAug E' d') MCells HCells)), *)
+(*     P Phi := fun P0 H0 => H0 (MCells Phi) (H Phi).  *)
 
-Arguments caseMAug {_ _ _ _ _ _ _ _} _.
+(* Arguments caseMAug {_ _ _ _ _ _ _ _} _. *)
 
 
 Definition FreeMA {F F' : Type} {n : nat} {aug : Aug F n} {aug' : Aug F' n}  {f : F -> F'} : aug - f -- aug' -> (FreeA aug -> FreeA aug').
 Proof.
-  intros Phi. destruct aug as [E d], aug' as [E' d'].
+  intros Phi. 
   simple refine (Pushout_rect _ _ _).
   - intro xf. exact (inl (f xf)).
   - intros. simple refine (inr _).
-    destruct Phi as [PhiE Phid] using caseMAug.
-    exact (PhiE (fst X), snd X ).
-  - intros [a a']. simpl.
-    destruct Phi as [PhiE Phid] using caseMAug. 
-    simple refine ((ap inl (Phid a a')^) @ _).
-    exact (incoh (PhiE a,a')).
+    exact (mkPair (ME Phi X,1) X,2).
+  - intro x. simpl.
+    simple refine ((ap inl (Md Phi x,1 x,2))^ @ _). 
+    exact (incoh (mkPair (ME Phi x,1) (x,2))).
 Defined.
 
 
 Definition ComposeMA {F F' F'' : Type} {n : nat} {f : F -> F'} {f' : F' -> F''} {aug : Aug F n} {aug' aug''} (G : MAug f aug aug') (G' : MAug f' aug' aug'') : MAug (compose f' f) aug aug''.
 Proof.
-  destruct aug as [E d]. destruct aug' as [E' d']. destruct aug'' as [E'' d''].
-  destruct G as [GE Gd] using caseMAug. destruct G' as [GE' Gd'] using caseMAug.
   simple refine (mkMAug _ _).
-  -  exact (compose GE' GE).
-  - simpl. intros. unfold compose. exact ((Gd' (GE e) x) @ (ap (fun W => f' W)  (Gd e x))).
+  - exact (compose (ME G') (ME G)).
+  - intros. unfold compose. exact ((Md G' (ME G e) x) @ (ap (fun W => f' W)  (Md G e x))).
 Defined.
 
+Lemma apap {A B : Type} (f : A -> B) {x y : A} {p q: x = y} (P : p = q) : ap f p = ap f q.
+Proof.
+  destruct P. reflexivity.
+Defined.
 
 Definition FreeComposeMA {F F' F'' : Type} {n : nat} {f : F -> F'} {f' : F' -> F''} {aug : Aug F n} {aug' aug''} (G : MAug f aug aug') (G' : MAug f' aug' aug'') : FreeMA (ComposeMA G G') = compose (FreeMA G') (FreeMA G).
 Proof.
-   destruct aug as [E d]. destruct aug' as [E' d']. destruct aug'' as [E'' d''].
-   destruct G as [GE Gd] using caseMAug. destruct G' as [GE' Gd'] using caseMAug.
-   simpl. 
-   unfold compose. simpl. simple refine ( (composeCPushout _ _)^).
-   - exact (fun x => (GE (fst x), snd x)).
-   - simpl. intros [a a'].  exact ((Gd a a')^).
-   - simpl. reflexivity.
-   - simpl. apply FunExtDep. intros [a a'].
-     exact ((concat_p1 _)^).
-   - simpl. apply FunExtDep. intros [a a']. 
-     simple refine (_ @ (concat_p1 _)^).
-     match goal with
-     | |- _ @ ?p = _ =>
-       simple refine ((ap (fun W => W @ p) (concat_ap_V _ _)) @  _);
-         simple refine ((ap (fun W => W ^ @ p) (ap_concat _ _ _)) @ _);
-         simple refine ((ap (fun W => W @ p) (concat_V _ _)) @ _);
-         simple refine ((assoc _ _ _)^ @ _ )
-     end.
-     match goal with
-     | |- (ap ?f (ap ?g ?p1)) ^ @ ?p2 = _ =>
-       simple refine ((ap (fun W => W^ @ p2) (ap_compose _ _ _)^) @ _)
-     end.
-     unfold compose.
-     match goal with
-     | |- _ = _ @ ?p =>
-       refine (_ @ ap (fun W => W @ p) (concat_ap_V _ _)^)
-     end.
-     match goal with
-     | |- _ = ?p @ (_ @ ?q) =>
-       exact (ap (fun W => p @ (W @ q)) (concat_ap_V inl _)^)
-     end.
+  apply funext. 
+  simple refine (Pushout_rect_dep _ _ _ _).
+  - reflexivity.
+  - reflexivity.
+  - intro x. apply transport_lemma. simpl.
+    rewrite concat_p1. unfold compose.
+    rewrite ap_compose. unfold FreeMA. unfold compose.
+    match goal with
+    | |- _ = ap (Pushout_rect ?g1 ?g2 ?H) (incoh x) => refine (_ @ (Pushout_rect_compute_coh (f1 := d aug) (f2 := fun x => mkPair x,1 (Faces n x,2)) (g1:= g1) (g2 := g2) (a := x))^)
+    end.
+    simpl. rewrite ap_concat.
+    match goal with
+    | |- ap ?F (ap (Pushout_rect ?g1 ?g2 ?H) (incoh x)) = _ => pose proof (Pushout_rect_compute_coh (f1 := d aug) (f2 := fun x => mkPair x,1 (Faces n x,2)) (g1 := g1) (g2 := g2) (H := H) (a := x))
+    end.
+    match goal with
+    | |- ap ?F ?u = ?v => refine (apap F H @ _); clear H
+    end.
+    rewrite ap_concat.
+    rewrite concat_ap_V.
+    match goal with
+    | |- (ap ?a1 (ap inl ?a2))^ @ _ = _ => change (ap a1 (ap inl a2)) with (compose (ap a1) (ap inl) a2); rewrite <- ap_compose
+    end.
+    unfold compose. simpl.
+    match goal with
+    | |- ?a1 @ ap (Pushout_rect ?g1 ?g2 ?H) (incoh ?y) = _ =>
+      refine (ap (fun T => a1 @ T) (Pushout_rect_compute_coh (f1 := d aug') (f2 := fun x => mkPair x,1 (Faces n x,2)) (g1 := g1) (g2 := g2) (H := H)) @ _)
+    end.
+    simpl. rewrite concat_V.
+    pose proof @ap_compose.
+    unfold compose in H. rewrite <- H.
+    now rewrite assoc.
 Defined.
 
 Inductive MPol : forall n : nat, (Pol n) -> (Pol n) -> Type :=
@@ -152,20 +196,16 @@ Arguments DiscM {_ _} _.
 Arguments ExtM {_ _ _ _ _} _ _.
 Arguments FreeM {_ _ _} _.
 
-Print caseS'.
 
-
-Definition case2 (n : nat) (p p' : Pol n)
+Definition case2 (n : nat) (p0 p1 : Pol n)
            (P : forall n : nat, Pol n -> Pol n -> Type)
-           (H0 : forall T T', P 0 (Disc T) (Disc T'))
-           (HS : forall n p aug p' aug', P (S n) (Ext p aug) (Ext p' aug')) :
-  P n p p' :=
-  match p with
-  |Disc T => (fun p' => case0 _ (H0 T) p')
-  |Ext p0 aug0 => (fun p' => caseS' _ p' _ (HS _ p0 aug0))
-  end p'.
-
-Check case2.
+           (H0 : forall T0 T1, P 0 (Disc T0) (Disc T1))
+           (HS : forall n p0 aug0 p1 aug1, P (S n) (Ext p0 aug0) (Ext p1 aug1)) :
+  P n p0 p1 :=
+  match p0 with
+  |Disc T0 => (fun p1 => case0 _ (H0 T0) p1)
+  |Ext p'0 aug'0 => (fun p1 => caseS' p1 _ (HS _ p'0 aug'0))
+  end p1.
 
   
 Definition caseM0 (T T' : Type)  (m : (Disc T) ~> (Disc T')):
@@ -184,7 +224,7 @@ Definition caseM0 (T T' : Type)  (m : (Disc T) ~> (Disc T')):
   | _ => tt
   end.
 
-Definition caseMS' (n : nat) (p p' : Pol n) (aug : Aug [p]* (S n)) (aug' : Aug [p']* (S n))
+Definition caseMS' (n : nat) (p p' : Pol n) (aug : Aug (Free p) (S n)) (aug' : Aug (Free p') (S n))
            (m : (Ext p aug) ~> (Ext p' aug')) :
   forall (P : (Ext p aug) ~> (Ext p' aug') -> Type)
     (HS : forall  (f : p ~> p') (Mf : MAug (FreeM f) aug aug'), P (ExtM f Mf)),
@@ -211,14 +251,14 @@ Proof.
     + econstructor. exact (compose h g).
     + exact 1.
   - simple refine (mkDPair _ _);
-      destruct p as [p' Ep] using (caseS' n);
-      destruct q as [q' Eq] using (caseS' n); destruct r as [r' Er] using (caseS' n);
+      destruct p as [p' Ep] using caseS';
+      destruct q as [q' Eq] using caseS'; destruct r as [r' Er] using caseS';
       destruct G as [G' GAug] using (caseMS' _ _ _ _ _); destruct  H as [H' HAug] using (caseMS' _ _ _ _ _).
     + unshelve econstructor.
       * exact (fstd (PolyComposeAndFree _ _ _ _ G' H')).
       * refine (transport (fun W => MAug W Ep Er) ((sndd (PolyComposeAndFree n p' q' r' G' H'))^) _).
         exact (ComposeMA GAug HAug).
-    + simpl.
+    + simpl. 
       simple refine (_ @ (FreeComposeMA _ _)).
       match goal with
       | |- ?f (transport ?P ?p ?u) = _ => exact (image_transport P p u _)
