pol/Adjunction.v
@@ -6,7 +6,7 @@ Require Import PolyMorphs.
 
 
 
-Definition EmptyA (n : nat) (T : Type) : Aug T n := mkAug False (fun x => False_rect _ (fst x)).
+Definition EmptyA (n : nat) (T : Type) : Aug T n := mkAug False (fun x => False_rect _ x,1).
 
 Definition Empty {n : nat} (p : Pol n) : Pol (S n) :=  Ext p (EmptyA (S n) (Free p)). 
 
@@ -20,25 +20,18 @@ Proof.
   destruct p. exact 1.
 Defined.
 
-Definition IdMA {n : nat} {T : Type} (aug : Aug T n)  : MAug (fun x => x) aug aug.
-Proof.
-  destruct aug as [E d].
-  unshelve econstructor.
-  - exact (fun x => x).
-  - simpl. reflexivity.
-Defined.
+Definition IdMA {n : nat} {T : Type} (aug : Aug T n)  : MAug (fun x => x) aug aug := mkMAug (fun x => x) (fun  _ _ => 1).
 
 Definition FreeIdMA {n : nat} {T : Type} (aug : Aug T n) : FreeMA (IdMA aug) = (fun x => x).
 Proof.
-  destruct aug as [E d]. apply funext.
+  apply funext.
   simple refine (eqMorphPushout _ _ _ ).
   - intro b1. simpl. reflexivity.
   - intro b2. simpl. destruct b2.  reflexivity.
   - simpl. intros [a a'].
-    simple refine (concat_1p _ @ _ @ (concat_p1 _)^). 
+    simple refine ( _ @ (concat_p1 _)^). 
     simple refine (ap_along_id _ @ _).
-    simple refine (_ @ Pushout_rect_compute_coh ^). simpl.
-    exact ((concat_1p _)^).
+    exact Pushout_rect_compute_coh ^. 
 Defined.
 
   
@@ -48,7 +41,7 @@ Proof.
   - simple refine (mkDPair _ _); intro p;  destruct p using case0.
     + econstructor.  exact (fun x => x).
     + exact 1.
-  -  simple refine (mkDPair _ _ ); intro p; destruct p using (caseS' n).
+  -  simple refine (mkDPair _ _ ); intro p; destruct p using caseS'.
     + unshelve econstructor.
       * exact (fstd (IdAndFreeM n) p).
       * match goal with
@@ -63,7 +56,6 @@ Defined.
 
 Definition EmptyMA (n : nat) (T : Type) (aug : Aug T n) : MAug (fun x => x) (EmptyA n T) aug.
 Proof.
-  destruct aug as [E d].
   simpl. unshelve econstructor. 
   - exact (False_rect _).
   - simpl. intro. contradiction.
@@ -89,13 +81,11 @@ Definition injectPol {n :nat} (p : Pol n) (aug : Aug (Free p) (S n)) : Free p ->
 
 Definition UnitA  {n : nat} {F T : Type}  (aug : Aug F n) (f : FreeA aug -> T) : MAug (injectA aug) aug (ForgetA f n).
 Proof.
-  destruct aug as [E d].
-  simpl.
   unshelve econstructor.
   - intro e. simple refine (mkPullB _ _ _).
-    + intro b. apply f. simpl. simple refine (inr _). exact (e,b).
-    + intro. simple refine (inl _). exact (d (e, X)).
-    + apply funext. intro. unfold nFaces. unfold compose. exact (ap f (incoh (e,x))^).
+    + intro b. apply f. simpl. simple refine (inr _). exact (mkPair e b).
+    + intro. simple refine (inl _). exact (d aug (mkPair e X)).
+    + apply funext. intro. unfold nFaces. unfold compose. exact (ap f (incoh (mkPair e x))^).
   - simpl. intros. reflexivity.
 Defined.
 
@@ -103,33 +93,24 @@ Definition UnitBisA {n : nat} {F : Type} (aug : Aug F (S n)) (f : F -> (Free (Fo
            (H : compose (Counit (FreeA aug) n) f = injectA aug):
   MAug f aug (ForgetA (Counit (FreeA aug) n) (S n)).
 Proof.
-  destruct aug.
-  simpl.
   unshelve econstructor.
-  -  intro e. simple refine (mkPullB _ _ _).
-     + intro x. exact (inr (e,x)).
-     + intro x.
-       match goal with
-       | |- context[ Pushout d ?f ] => change (Pushout d f) with (FreeA (mkAug _ d))
-       end.
-       apply f. exact (d (e, x)).
+  -  intro e. simpl. simple refine (mkPullB _ _ _).
+     + intro x. exact (inr (mkPair e x)).
+     + intro x. simpl.
+       apply f. exact (d aug (mkPair e x)).
      + unfold nFaces. unfold compose. apply funext. intro x.
-       match goal with
-       | |- context[ Pushout d ?f ] => change (Pushout d f) with (FreeA (mkAug _ d))
-       end.
-       simple refine (_ @ (ap (fun W => W (d (e, x))) H^)).
-       unfold injectA. unfold compose. unfold FreeEmptyA. unfold EmptyMA. simpl. exact ((incoh (e, x))^).
-  - simpl. reflexivity.
+       simple refine (_ @ (ap (fun W => W (d aug (mkPair e x))) H^)).
+       exact ((incoh (mkPair e x))^).
+  - reflexivity.
 Defined.
 
 Definition TriangleA  {n : nat} {F T : Type}  (aug : Aug F n) (f : FreeA aug -> T) : compose (CounitA n f) (FreeMA (UnitA aug f)) = f.
 Proof.
-  destruct aug as [E d].
   apply funext. simple refine (eqMorphPushout _ _ _).
-  - intro b1. unfold compose. simpl. unfold injectA. unfold compose. simpl. reflexivity.
+  - reflexivity.
   - intro b2. unfold compose. simpl. destruct b2. reflexivity.
   - intros [a a']. simpl.
-    simple refine (concat_1p _ @ _ @ (concat_p1 _)^).
+    simple refine ( _ @ (concat_p1 _)^).
     match goal with
     | |- _ = ap (compose ?f ?g) ?p => simple refine (_ @ (ap_compose g f p)^)
     end.
@@ -138,9 +119,6 @@ Proof.
     | |- _ = ap ?f _ => simple refine (_ @ ap (ap f) Pushout_rect_compute_coh^)
     end.
     simpl.
-    match goal with
-    | |- _ = ap ?f (1 @ ?p)  =>  simple refine (_ @ (ap (fun W => ap f W) (concat_1p p)^))
-    end.
     unfold CounitA.
     simple refine (_ @ Pushout_rect_compute_coh^). simpl.
     simple refine (_ @ (concat_ap_V _ _)^).
@@ -158,38 +136,31 @@ Lemma TriangleABis {n : nat} {F : Type} (aug : Aug F (S n)) (f : F -> (Free (For
            compose (CounitA (S n) (Counit (FreeA aug) n))
                    (FreeMA (UnitBisA aug f H)) = (fun x : FreeA aug => x).
 Proof.
-  destruct aug. apply funext. simple refine (eqMorphPushout _ _ _).
+  apply funext. simple refine (eqMorphPushout _ _ _).
   - intro b1. unfold compose. simpl. exact (ap (fun W => W b1) H).
   - intro b2. unfold compose. simpl. destruct b2. reflexivity.
-  - intros [a a']. unfold compose. simpl.
+  - intros a. unfold compose. simpl.
+    simple refine (_ @ (concat_p1 _)^).
     match goal with
-    | |- context[ Pushout d ?f ] => change (Pushout d f) with (FreeA (mkAug _ d))
-    end.
-    simple refine (_ @ (concat_p1 _)^). simpl.
-    match goal with
-    | |- _ = ap (fun x => CounitA ?a1 ?a2  (@?W x)) (incoh (a, a')) =>
-      change (ap (fun x => CounitA a1 a2 (W x)) (incoh (a, a'))) with
-          (ap (compose (CounitA a1 a2) W) (incoh (a, a')));
-        simple refine (_ @ (ap_compose W (CounitA a1 a2) (incoh (a, a')))^)
-    end. unfold compose.
+    | |- _ = ap (fun x => CounitA ?a1 ?a2  (@?W x)) (incoh a) =>
+      change (ap (fun x => CounitA a1 a2 (W x)) (incoh a)) with
+          (ap (compose (CounitA a1 a2) W) (incoh a));
+        simple refine (_ @ (ap_compose W (CounitA a1 a2) (incoh a))^)
+    end. unfold compose. unfold CounitA.
     match goal with
     | |- _ = ap ?f _  => simple refine (_ @ (ap (fun W => ap f W) Pushout_rect_compute_coh^))
-    end.
-    simpl.
+    end. simpl.
     match goal with
-    | |- _ = ap ?f (1 @ ?p)  => simple refine (_ @ (ap (fun W => ap f W) (concat_1p p )^))
+    | |- _ = ap (Pushout_rect ?a1 ?a2 ?a3) (incoh ?a4) =>
+      simple refine (_ @ (Pushout_rect_compute_coh (f1 := (fun x  => pi2 x,1 x,2)) )^)
     end.
-    simple refine (_ @ Pushout_rect_compute_coh^).
     simpl.
     match goal with
     | |- _ = ap ?f ?p ^ => simple refine (_ @ (concat_ap_V f p)^)
     end.
     match goal with
-    | |- _ = (ap (fun W => W a') (funext ?p))^ => 
-      simple refine (_ @ (ap (fun W => W^) (funextcompute p a')^))
-    end.
-    match goal with
-    | |- context[ Pushout d ?f ] => change (Pushout d f) with (FreeA (mkAug _ d))
+    | |- _ = (ap (fun W => W a,2) (funext ?p))^ => 
+      simple refine (_ @ (ap (fun W => W^) (funextcompute p a,2)^))
     end.
     match goal with
     | |- ?p @ _ = _ => simple refine ((ap (fun W => p @ W) (ap_id _)) @ _)
@@ -203,7 +174,6 @@ Proof.
     end.
 Defined.
 
-Definition test (n : nat) (p : Pol n) :  (@Free n p) = (Polygraphs.Free p) := 1.
 
 Fixpoint UnitPol {n : nat} (p : Pol n) {struct n} : {f :  MPol p (Forget (Free p) n) |
                                                               compose (Counit (Free p) n) (FreeM f) = (fun x => x)}.
@@ -212,7 +182,7 @@ Proof.
   - simple refine (mkDPair _ _).
     + destruct p using case0. econstructor. exact (fun x => x).
     + destruct p using case0. exact 1.
-  - simple refine (mkDPair _ _); destruct p as [p aug] using (caseS' n).
+  - simple refine (mkDPair _ _); destruct p as [p aug] using caseS'.
     + simpl. unshelve econstructor. 
       * exact (ComposeM (fstd (UnitPol n p)) (ForgetM n (injectPol p aug) ) ).
       * simpl.  simple refine (UnitBisA _ _ _).
